Fix case-syntax in whileLemmas.

lib/whileLemmasScript.sml
@@ -69,12 +69,12 @@ METIS_TAC []
 ]);
 
 val owhile_EQ_SOME = store_thm(
-"owhile_EQ_SOME", 
+"owhile_EQ_SOME",
 ``(?s'.owhile C f s = SOME s') = terminates (C, f, s)``,
 SRW_TAC [] [EQ_IMP_THM] THEN
  METIS_TAC [optionTheory.NOT_SOME_NONE,optionTheory.option_nchotomy,owhile_EQ_NONE])
 
-val owhileEndCond = store_thm ("owhileEndCond", 
+val owhileEndCond = store_thm ("owhileEndCond",
 ``!s'.(owhile C f s = SOME s') ==> ~ C s'``,
 FULL_SIMP_TAC (srw_ss()) [owhile_def,owhile_EQ_SOME,if_rw_SOMEeqSOME] THEN
 STRIP_TAC THEN
@@ -82,10 +82,10 @@ numLib.LEAST_ELIM_TAC THEN SRW_TAC [][] THEN METIS_TAC []
 )
 
 val nthStateProp = store_thm ("nthStateProp",
-``(!x. P x /\ C x ==> P (f x)) ==> 
+``(!x. P x /\ C x ==> P (f x)) ==>
 !n s.P s /\ (!m.m < n ==> C (FUNPOW f m s)) ==> P (FUNPOW f n s)``,
 STRIP_TAC THEN
-Induct_on `n` THEN 
+Induct_on `n` THEN
 SRW_TAC [] [FUNPOW] THEN
 FIRST_ASSUM MATCH_MP_TAC THEN
 `P (f s)`  by METIS_TAC [DECIDE ``0 < SUC n``,FUNPOW] THEN
@@ -93,7 +93,7 @@ SRW_TAC [] [] THEN
 METIS_TAC [DECIDE ``m < n ==> SUC m < SUC n``,FUNPOW])
 
 
-val owhileEndState = store_thm ("owhileEndState", 
+val owhileEndState = store_thm ("owhileEndState",
 ``((owhile C f s = SOME s') /\ (!x.P x /\ C x ==> P (f x)) /\ P s) ==> P s'``,
 SRW_TAC [] [owhile_def,owhile_EQ_SOME] THEN
 numLib.LEAST_ELIM_TAC THEN SRW_TAC [][] THENL[
@@ -104,34 +104,34 @@ METIS_TAC [nthStateProp]]
 
 (* mwhile G C can have three different results:
     NONE - went into an infinite loop
-    SOME NONE - aborted (body returned NONE on some state) 
-    SOME (SOME s) - successful termination in state s 
+    SOME NONE - aborted (body returned NONE on some state)
+    SOME (SOME s) - successful termination in state s
 *)
 
 val mwhile = Define`
-  mwhile g f s = 
-    owhile (\opt. case opt of NONE -> F || SOME s -> g s)
-           (\opt. case opt of NONE -> NONE 
-                           || SOME s -> f s)
+  mwhile g f s =
+    owhile (\opt. case opt of NONE => F | SOME s => g s)
+           (\opt. case opt of NONE => NONE
+                           | SOME s => f s)
            (SOME s)
 `;
 
 val mwhile_COND = store_thm(
   "mwhile_COND",
-  ``mwhile g f s = 
-           if g s then 
-              case f s of 
-                NONE -> SOME NONE
-             || SOME s' -> mwhile g f s'
+  ``mwhile g f s =
+           if g s then
+              case f s of
+                NONE => SOME NONE
+             | SOME s' => mwhile g f s'
            else SOME (SOME s)``,
   SRW_TAC [][mwhile] THENL [
-    CONV_TAC (LAND_CONV (ONCE_REWRITE_CONV [owhile_thm])) THEN 
-    SRW_TAC [][] THEN 
-    Cases_on `f s` THEN SRW_TAC [][] THEN 
-    CONV_TAC (LAND_CONV (ONCE_REWRITE_CONV [owhile_thm])) THEN 
+    CONV_TAC (LAND_CONV (ONCE_REWRITE_CONV [owhile_thm])) THEN
+    SRW_TAC [][] THEN
+    Cases_on `f s` THEN SRW_TAC [][] THEN
+    CONV_TAC (LAND_CONV (ONCE_REWRITE_CONV [owhile_thm])) THEN
     SRW_TAC [][],
 
-    CONV_TAC (LAND_CONV (ONCE_REWRITE_CONV [owhile_thm])) THEN 
+    CONV_TAC (LAND_CONV (ONCE_REWRITE_CONV [owhile_thm])) THEN
     SRW_TAC [][]
   ]);
 
@@ -140,10 +140,10 @@ val mwhile_COND = store_thm(
 (*
 val mwhile_EQ_NONE = store_thm(
 "mwhile_EQ_NONE",
-``!C f s.(mwhile C f s = NONE) = 
+``!C f s.(mwhile C f s = NONE) =
 ~terminates ((\opt. case opt of NONE -> T || SOME x -> C x),
              (\opt. case opt of NONE -> NONE || SOME x -> f x), SOME s)``,
-SRW_TAC [][mwhile, terminates_def, owhile_def] THEN 
+SRW_TAC [][mwhile, terminates_def, owhile_def] THEN
 Cases_on `FUNPOW (\opt. case opt of NONE -> NONE || SOME s -> f s) n (SOME s)` THEN
 SRW_TAC [][] THEN
 Q.EXISTS_TAC `n`  THEN
@@ -154,7 +154,7 @@ METIS_TAC [NEW_THEORY])
 
 (*
 val mwhile_EQ_SOME = store_thm(
-"mwhile_EQ_SOME", 
+"mwhile_EQ_SOME",
 ``(?s'.mwhile C f s = SOME s') = terminates ((\opt. case opt of NONE -> T || SOME x -> C x),
                                   (\opt. case opt of NONE -> NONE || SOME x -> f x), SOME s)``,
 SRW_TAC [] [EQ_IMP_THM] THEN
@@ -162,10 +162,10 @@ SRW_TAC [] [EQ_IMP_THM] THEN
 mwhile_EQ_NONE])
 *)
 
-val mwhileEndCond = store_thm ("mwhileEndCond", 
+val mwhileEndCond = store_thm ("mwhileEndCond",
 ``(mwhile C f s = SOME (SOME s')) ==> ~ C s'``,
 SRW_TAC [] [mwhile] THEN
-METIS_TAC [owhileEndCond, optionTheory.option_case_def]) 
+METIS_TAC [owhileEndCond, optionTheory.option_case_def])
 
 
 
@@ -178,7 +178,7 @@ Q.MATCH_ABBREV_TAC `(owhile CC ff (SOME s) = SOME (SOME s')) /\
 (!x y. P x /\ C x /\ (f x = SOME y) ==> P y) /\
 P s ==> P s'` THEN
 STRIP_TAC THEN
-Q.ABBREV_TAC `PP = \x. case x of NONE -> T || SOME s -> P s` THEN
+Q.ABBREV_TAC `PP = \x. case x of NONE => T | SOME s => P s` THEN
 `(!x. PP x /\ CC x ==> PP (ff x)) /\ PP (SOME s) ==> PP (SOME s')`
 by METIS_TAC [owhileEndState] THEN
 markerLib.UNABBREV_ALL_TAC THEN
